theories/heap_lang/adequacy.v
@@ -4,22 +4,22 @@ From iris_time.heap_lang Require Import proofmode notation.
 From iris.proofmode Require Import tactics.
 Set Default Proof Using "Type".
 
-Class heapPreG Σ := HeapPreG {
-  heap_preG_iris :> invPreG Σ;
-  heap_preG_heap :> gen_heapPreG loc val Σ
+Class heapGpreS Σ := HeapGpreS {
+  heap_preG_iris :> invGpreS Σ;
+  heap_preG_heap :> gen_heapGpreS loc val Σ
 }.
 
 Definition heapΣ : gFunctors := #[invΣ; gen_heapΣ loc val].
-Instance subG_heapPreG {Σ} : subG heapΣ Σ → heapPreG Σ.
+Instance subG_heapPreG {Σ} : subG heapΣ Σ → heapGpreS Σ.
 Proof. solve_inG. Qed.
 
-Definition heap_adequacy Σ `{heapPreG Σ} s e σ φ :
-  (∀ `{heapG Σ}, ⊢ WP e @ s; ⊤ {{ v, ⌜φ v⌝ }}) →
+Definition heap_adequacy Σ `{heapGpreS Σ} s e σ φ :
+  (∀ `{heapGS Σ}, ⊢ WP e @ s; ⊤ {{ v, ⌜φ v⌝ }}) →
   adequate s e σ (λ v _, φ v).
 Proof.
   intros Hwp; eapply (wp_adequacy _ _); iIntros (??) "".
   iMod (gen_heap_init σ) as (?) "[Hh _]".
   iModIntro.
   iExists (λ σ κs, (gen_heap_interp σ)%I), (λ _, True%I). iFrame.
-  iApply (Hwp (HeapG _ _ _)).
+  iApply (Hwp (HeapGS _ _ _)).
 Qed.
