theories/heap_lang/proofmode.v
@@ -6,7 +6,7 @@ From iris_time.heap_lang Require Import notation.
 Set Default Proof Using "Type".
 Import uPred.
 
-Lemma tac_wp_expr_eval `{heapG Σ} Δ s E Φ e e' :
+Lemma tac_wp_expr_eval `{heapGS Σ} Δ s E Φ e e' :
   (∀ (e'':=e'), e = e'') →
   envs_entails Δ (WP e' @ s; E {{ Φ }}) → envs_entails Δ (WP e @ s; E {{ Φ }}).
 Proof. by intros ->. Qed.
@@ -22,7 +22,7 @@ Tactic Notation "wp_expr_eval" tactic(t) :=
 
 Ltac wp_expr_simpl := wp_expr_eval simpl.
 
-Lemma tac_wp_pure `{heapG Σ} Δ Δ' s E K e1 e2 φ n Φ :
+Lemma tac_wp_pure `{heapGS Σ} Δ Δ' s E K e1 e2 φ n Φ :
   PureExec φ n e1 e2 →
   φ →
   MaybeIntoLaterNEnvs n Δ Δ' →
@@ -35,7 +35,7 @@ Proof.
   rewrite HΔ' -lifting.wp_pure_step_later //.
 Qed.
 
-Lemma tac_wp_value `{heapG Σ} Δ s E Φ v :
+Lemma tac_wp_value `{heapGS Σ} Δ s E Φ v :
   envs_entails Δ (Φ v) → envs_entails Δ (WP (Val v) @ s; E {{ Φ }}).
 Proof. rewrite envs_entails_eq=> ->. by apply wp_value. Qed.
 
@@ -95,7 +95,7 @@ Tactic Notation "wp_inj" := wp_pure (InjL _) || wp_pure (InjR _).
 Tactic Notation "wp_pair" := wp_pure (Pair _ _).
 Tactic Notation "wp_closure" := wp_pure (Rec _ _ _).
 
-Lemma tac_wp_bind `{heapG Σ} K Δ s E Φ e f :
+Lemma tac_wp_bind `{heapGS Σ} K Δ s E Φ e f :
   f = (λ e, fill K e) → (* as an eta expanded hypothesis so that we can `simpl` it *)
   envs_entails Δ (WP e @ s; E {{ v, WP f (Val v) @ s; E {{ Φ }} }})%I →
   envs_entails Δ (WP fill K e @ s; E {{ Φ }}).
@@ -118,7 +118,7 @@ Tactic Notation "wp_bind" open_constr(efoc) :=
 
 (** Heap tactics *)
 Section heap.
-Context `{WordSize, heapG Σ}.
+Context `{WordSize, heapGS Σ}.
 Implicit Types P Q : iProp Σ.
 Implicit Types Φ : val → iProp Σ.
 Implicit Types Δ : envs (uPredI (iResUR Σ)).
